axiomatic.v
@@ -80,23 +80,23 @@ of the previously defined notions together. We require both the program and
 the memory to contain no locks at the start. Also, we require all locks to be
 released in the end, as each statement that contains an expression always has
 a sequence point in the end. *)
-Inductive ax_stmt_post' `{Env K} (Pd : dassert K) (s : stmt K)
-    (Γ : env K) (Δ : memenv K) (ρ : stack K) : focus K → mem K → Prop :=
+Inductive ax_stmt_post' `{Env K} (Pd : dassert K) (s : stmt K) (Γ : env K)
+    (Δ : memenv K) (ρ : stack K) (n : nat) : focus K → mem K → Prop :=
   mk_ax_stmt_post d m :
     direction_out d s →
     mem_locks m = ∅ →
-    assert_holds (Pd d) Γ Δ ρ (cmap_erase m) →
-    ax_stmt_post' Pd s Γ Δ ρ (Stmt d s) m.
+    assert_holds (Pd d) Γ Δ ρ n (cmap_erase m) →
+    ax_stmt_post' Pd s Γ Δ ρ n (Stmt d s) m.
 Program Definition ax_stmt_post `{Env K}
     (Pd : dassert K) (s : stmt K) : ax_assert K := {|
   ax_assert_holds := ax_stmt_post' Pd s
 |}.
 Next Obligation.
-  intros ?? Pd s Γ1 Γ2 Δ1 Δ2 ρ φ m ???; destruct 1 as [d m' ???];
+  intros ?? Pd s Γ1 Γ2 Δ1 Δ2 ρ n φ m ????; destruct 1 as [d m' ???];
     constructor; eauto using assert_weaken, cmap_erase_valid.
 Qed.
 Next Obligation.
-  intros ?? Pd s Γ δ Δ ρ φ m m' [d m'' ???] [? p]; inv_rcstep.
+  intros ?? Pd s Γ δ Δ n ρ φ m m' [d m'' ???] [? p]; inv_rcstep.
 Qed.
 Definition ax_stmt_packed `{EnvSpec K} (Γ : env K) (δ : funenv K)
     (Pd : dassert K) (s : stmt K) : Prop := ∀ Δ n ρ d m cmτ,
@@ -106,7 +106,7 @@ Definition ax_stmt_packed `{EnvSpec K} (Γ : env K) (δ : funenv K)
   direction_in d s →
   (Γ,Δ,ρ.*2) ⊢ s : cmτ →
   ✓{Δ}* ρ →
-  assert_holds (Pd d) Γ Δ ρ (cmap_erase m) →
+  assert_holds (Pd d) Γ Δ ρ n (cmap_erase m) →
   ax_graph ax_disjoint_cond (ax_stmt_post Pd s) Γ δ Δ ρ n [] (Stmt d s) m.
 Instance: Params (@ax_stmt_packed) 5.
 Notation "Γ \ δ \ P ⊨ₚ s" :=
@@ -143,69 +143,70 @@ Arguments InExpr {_} _ _.
 Arguments InFun {_} _.
 
 Inductive ax_expr_cond_frame `{Env K}
-     (ρ : stack K) (A : assert K) (Γ : env K) (Δ : memenv K)
-     (k : ctx K) (φ : focus K) (m m' : mem K) : ax_expr_frame K → Prop :=
+     (ρ : stack K) (A : assert K) (Γ : env K) (Δ : memenv K) (k : ctx K) 
+     (n : nat) (φ : focus K) (m m' : mem K) : ax_expr_frame K → Prop :=
   | ax_frame_in_expr mA mf :
      m' = m ∪ mf ∪ mA → ✓{Γ,Δ} mf → ✓{Γ,Δ} mA →
      ⊥ [m; mf; mA] → k = [] → cmap_erased mA → mem_locks mA = ∅ →
-     assert_holds A Γ Δ ρ mA →
-     ax_expr_cond_frame ρ A Γ Δ k φ m m' (InExpr mf mA)
+     assert_holds A Γ Δ ρ n mA →
+     ax_expr_cond_frame ρ A Γ Δ k n φ m m' (InExpr mf mA)
   | ax_frame_in_fun mf :
      m' = m ∪ mf → ✓{Γ,Δ} mf →
      ⊥ [m; mf] → k ≠ [] →
-     ax_expr_cond_frame ρ A Γ Δ k φ m m' (InFun mf).
+     ax_expr_cond_frame ρ A Γ Δ k n φ m m' (InFun mf).
 Inductive ax_expr_cond_unframe `{Env K}
-     (ρ : stack K) (A : assert K) (Γ : env K) (Δ : memenv K)
-     (k : ctx K) (φ : focus K) (m m' : mem K) : ax_expr_frame K → Prop :=
+     (ρ : stack K) (A : assert K) (Γ : env K) (Δ : memenv K) (k : ctx K)
+     (n : nat) (φ : focus K) (m m' : mem K) : ax_expr_frame K → Prop :=
   | ax_unframe_expr_to_expr mA mf :
      m' = m ∪ mf ∪ mA → ⊥ [m; mf; mA] → k = [] →
-     ax_expr_cond_unframe ρ A Γ Δ k φ m m' (InExpr mf mA)
+     ax_expr_cond_unframe ρ A Γ Δ k n φ m m' (InExpr mf mA)
   | ax_unframe_fun_to_expr mA mf :
      m' = m ∪ mf ∪ mA → ⊥ [m; mf; mA] → k = [] →
      cmap_erased mA → mem_locks mA = ∅ →
-     assert_holds A Γ Δ ρ mA → 
-     ax_expr_cond_unframe ρ A Γ Δ k φ m m' (InFun mf)
+     assert_holds A Γ Δ ρ n mA → 
+     ax_expr_cond_unframe ρ A Γ Δ k n φ m m' (InFun mf)
   | ax_unframe_expr_to_fun m'' mA mf :
      m = m'' ∪ mA → m' = m'' ∪ mf ∪ mA → ⊥ [m''; mf; mA] → k ≠ [] →
-     ax_expr_cond_unframe ρ A Γ Δ k φ m m' (InExpr mf mA)
+     ax_expr_cond_unframe ρ A Γ Δ k n φ m m' (InExpr mf mA)
   | ax_unframe_fun_to_fun mf :
      m' = m ∪ mf → ⊥ [m; mf] → k ≠ [] →
-     ax_expr_cond_unframe ρ A Γ Δ k φ m m' (InFun mf).
+     ax_expr_cond_unframe ρ A Γ Δ k n φ m m' (InFun mf).
 Program Definition ax_expr_cond `{EnvSpec K} (ρ : stack K)
     (A : assert K) : ax_frame_cond K (ax_expr_frame K) := {|
   frame := ax_expr_cond_frame ρ A;
   unframe := ax_expr_cond_unframe ρ A
 |}.
 Next Obligation.
-  intros ??? ρ A Γ Δ k φ m m' ??;
+  intros ??? ρ A Γ Δ k n φ m m' ??;
     destruct 1; subst; auto using cmap_union_valid_2.
 Qed.
 Next Obligation.
-  intros ??? ρ A Γ Δ k φ m m' ??; destruct 1; subst;
+  intros ??? ρ A Γ Δ k n φ m m' ??; destruct 1; subst;
     rewrite ?cmap_union_valid; intuition.
 Qed.
 
 Definition ax_expr_funframe `{Env K} (Γ : env K) (Δ : memenv K)
-    (A : assert K) (ρ : stack K) (m : mem K) := ∃ mA,
+    (A : assert K) (ρ : stack K) (n : nat) (m : mem K) := ∃ mA,
   ⊥ [mA; m] ∧ ✓{Γ,Δ} mA ∧ cmap_erased mA ∧ mem_locks mA = ∅ ∧
-  assert_holds A Γ Δ ρ mA.
-Inductive ax_expr_post' `{Env K} (Q : lrval K → assert K) (τlr : lrtype K)
-    (Γ : env K) (Δ : memenv K) (ρ : stack K) : focus K → mem K → Prop :=
+  assert_holds A Γ Δ ρ n mA.
+Inductive ax_expr_post' `{Env K} (Q : lrval K → assert K)
+    (τlr : lrtype K) (Γ : env K) (Δ : memenv K) (ρ : stack K)
+    (n : nat) : focus K → mem K → Prop :=
   mk_ax_expr_post ν Ω m :
     (Γ,Δ) ⊢ ν : τlr →
     mem_locks m = Ω →
-    assert_holds (Q ν) Γ Δ ρ (cmap_erase m) →
-    ax_expr_post' Q τlr Γ Δ ρ (Expr (%#{Ω} ν)) m.
+    assert_holds (Q ν) Γ Δ ρ n (cmap_erase m) →
+    ax_expr_post' Q τlr Γ Δ ρ n (Expr (%#{Ω} ν)) m.
 Program Definition ax_expr_post `{EnvSpec K}
     (Q : lrval K → assert K) (τlr : lrtype K) : ax_assert K := {|
   ax_assert_holds := ax_expr_post' Q τlr
 |}.
 Next Obligation.
-  intros ??? Q τlr Γ1 Γ2 Δ1 Δ2 ρ φ m ???; destruct 1; constructor;
+  intros ??? Q τlr Γ1 Γ2 Δ1 Δ2 ρ n φ m ????; destruct 1; constructor;
     eauto using assert_weaken, cmap_erase_valid, lrval_typed_weaken.
 Qed.
 Next Obligation.
-  intros ??? Q τlr Γ δ Δ ρ φ m m' [d m'' ???] [? p]; inv_rcstep.
+  intros ??? Q τlr Γ δ Δ ρ n φ m m' [d m'' ???] [? p]; inv_rcstep.
 Qed.
 Definition ax_expr `{EnvSpec K} (Γ : env K) (δ : funenv K) (A P : assert K)
     (e : expr K) (Q : lrval K → assert K) : Prop := ∀ Δ n ρ m τlr,
@@ -215,8 +216,8 @@ Definition ax_expr `{EnvSpec K} (Γ : env K) (δ : funenv K) (A P : assert K)
   (Γ,Δ,ρ.*2) ⊢ e : τlr →
   locks e = ∅ →
   ✓{Δ}* ρ →
-  ax_expr_funframe Γ Δ A ρ m →
-  assert_holds P Γ Δ ρ (cmap_erase m) →
+  ax_expr_funframe Γ Δ A ρ n m →
+  assert_holds P Γ Δ ρ n (cmap_erase m) →
   ax_graph (ax_expr_cond ρ A) (ax_expr_post Q τlr) Γ δ Δ ρ n [] (Expr e) m.
 Instance: Params (@ax_expr) 5.
 Notation "Γ \ δ \ A ⊨ₑ {{ P }} e {{ Q }}" :=
@@ -245,6 +246,7 @@ Implicit Types S : state K.
 Hint Immediate cmap_valid_memenv_valid.
 Hint Resolve cmap_empty_valid cmap_erased_empty mem_locks_empty.
 Hint Resolve cmap_union_valid_2 cmap_erase_valid.
+Hint Extern 1 (_ ≤ _) => omega.
 
 Global Instance directed_pack_proper `{!@Equivalence A R} :
   Proper (R ==> R ==> pointwise_relation _ R ==> pointwise_relation _ R ==>
@@ -261,8 +263,9 @@ Proof.
               (ax_stmt_packed Γ δ)).
   { intros help. by split; apply help. }
   intros Pd Qd HPQ ?? -> Hax ?????????????.
-  eapply ax_weaken; [| |eapply Hax| | |]; eauto; [eapply HPQ; eauto|].
-  destruct 3; constructor; auto. eapply HPQ; eauto using indexes_valid_weaken.
+  eapply ax_weaken with ax_disjoint_cond (ax_stmt_post Pd y) n; eauto.
+  { eapply Hax, HPQ; eauto. }
+  destruct 2; constructor; auto. eapply HPQ; eauto using indexes_valid_weaken.
 Qed.
 Lemma ax_stmt_top_unfold Γ δ P (Q : val _ → assert _) s :
   Γ\ δ ⊨ₛ {{ P }} s {{ Q }} ↔
@@ -284,19 +287,21 @@ Proof.
   unfold ax_stmt_top, dassert_pack_top. by rewrite HP, HQ.
 Qed.
 
-Lemma ax_expr_funframe_emp Γ Δ ρ m : ✓{Γ,Δ} m → ax_expr_funframe Γ Δ emp ρ m.
+Lemma ax_expr_funframe_emp Γ Δ ρ n m : ✓{Γ,Δ} m → ax_expr_funframe Γ Δ emp ρ n m.
 Proof. by eexists ∅; split_ands; eauto. Qed.
 Hint Resolve ax_expr_funframe_emp.
-Lemma ax_expr_funframe_weaken Γ Δ A ρ m1 m2 :
-  ax_expr_funframe Γ Δ A ρ m2 → m1 ⊆ m2 → ax_expr_funframe Γ Δ A ρ m1.
+Lemma ax_expr_funframe_weaken Γ Δ A ρ n1 n2 m1 m2 :
+  ✓ Γ → ✓{Δ}* ρ →
+  ax_expr_funframe Γ Δ A ρ n1 m2 → m1 ⊆ m2 → n2 ≤ n1 →
+  ax_expr_funframe Γ Δ A ρ n2 m1.
 Proof.
-  intros (mA&?&?&?) Hm12; exists mA; split; auto.
+  intros ?? (mA&?&?&?&?&?) Hm12; exists mA; split_ands; eauto using assert_weaken.
   by rewrite <-(sep_subseteq_disjoint_le m1) by eauto.
 Qed.
 Lemma ax_disjoint_expr_compose_diagram Γ ρ A Ek :
   ax_compose_diagram ax_disjoint_cond (ax_expr_cond ρ A) Γ [Ek].
 Proof.
-  intros Δ k φ a m m' ?; simpl. destruct 1; subst; [discriminate_list_equality|].
+  intros Δ k n φ a m m' ?; simpl. destruct 1; subst; [discriminate_list_equality|].
   exists mf; split_ands; auto; intros Δ' k' φ' m2 m2' ?? [-> ?].
   constructor; trivial; intro; discriminate_list_equality.
 Qed.
@@ -304,7 +309,7 @@ Hint Resolve ax_disjoint_expr_compose_diagram.
 Lemma ax_expr_disjoint_compose_diagram Γ ρ k :
   ax_compose_diagram (ax_expr_cond ρ emp%A) ax_disjoint_cond Γ k.
 Proof.
-  intros Δ k' φ m m' mf ? (->&?&?); simpl; destruct (decide (k' = [])) as [->|].
+  intros Δ k' φ n m m' mf ? (->&?&?); simpl; destruct (decide (k' = [])) as [->|].
   * exists (InExpr mf ∅). split.
     { by constructor; rewrite ?sep_right_id by auto;
         eauto using mem_locks_empty, cmap_empty_valid, cmap_erased_empty. }
@@ -318,7 +323,7 @@ Hint Resolve ax_expr_disjoint_compose_diagram.
 Lemma ax_expr_cond_frame_diagram_simple Γ ρ B mf :
   ax_frame_diagram (ax_expr_cond ρ B) (ax_expr_cond ρ B) Γ mf.
 Proof.
-  intros Δ k φ m m' ?; destruct 4 as [mA mf'|mf']; subst.
+  intros Δ k φ n m m' ?; destruct 4 as [mA mf'|mf']; subst.
   * simplify_mem_disjoint_hyps; exists (InExpr (mf ∪ mf') mA); split.
     { constructor; auto. by rewrite sep_associative by auto. }
     intros Δ' k' φ' m2 m2'.
@@ -347,28 +352,30 @@ Proof.
     pointwise_relation _ (≡{Γ}) ==> impl) (ax_expr Γ δ)).
   { intros help. by split; apply help. }
   intros A1 A2 HA P1 P2 HP ?? -> Q1 Q2 HQ Hax ??????????? (?&?&?&?&?&?) ?.
-  eapply ax_weaken; [| |apply Hax| | |]; eauto.
-  * econstructor; split_ands; eauto. apply HA; eauto.
-  * apply HP; eauto.
-  * destruct 3; constructor; auto. apply HA; eauto using indexes_valid_weaken.
-  * destruct 3; subst; simplify_mem_disjoint_hyps;
+  eapply ax_weaken with (ax_expr_cond ρ A1) (ax_expr_post Q1 τlr) n; eauto.
+  * apply Hax, HP; eauto.
+    econstructor; split_ands; eauto. apply HA; eauto.
+  * destruct 2; constructor; auto. apply HA; eauto using indexes_valid_weaken.
+  * destruct 2; subst; simplify_mem_disjoint_hyps;
      econstructor (first [by eauto|apply HA; eauto using indexes_valid_weaken]).
-  * destruct 3; constructor; auto. apply HQ; eauto using indexes_valid_weaken.
+  * destruct 2; constructor; auto. apply HQ; eauto using indexes_valid_weaken.
 Qed.
 
-Lemma ax_expr_post_expr_nf Γ Q Δ ρ m e τlr :
-  ax_expr_post' Q τlr Γ Δ ρ (Expr e) m → is_nf e.
+Lemma ax_expr_post_expr_nf Γ Q Δ ρ n m e τlr :
+  ax_expr_post' Q τlr Γ Δ ρ n (Expr e) m → is_nf e.
 Proof. by inversion 1. Qed.
 Lemma ax_expr_lrval Γ δ A (P : lrval K → assert K) Δ ρ n ν Ω m τlr :
-  ✓{Γ,Δ} m → ax_expr_funframe Γ Δ A ρ m →
+  ✓{Γ,Δ} m → ax_expr_funframe Γ Δ A ρ n m →
   ax_graph (ax_expr_cond ρ A)
     (ax_expr_post P τlr) Γ δ Δ ρ (S n) [] (Expr (%#{Ω} ν)%E) m →
-  assert_holds (P ν) Γ Δ ρ (cmap_erase m) ∧ mem_locks m = Ω ∧ (Γ,Δ) ⊢ ν : τlr.
+  assert_holds (P ν) Γ Δ ρ (S n) (cmap_erase m)
+  ∧ mem_locks m = Ω ∧ (Γ,Δ) ⊢ ν : τlr.
 Proof.
   intros ? (mA&?&?&?&?&?);
-    inversion 1 as [|??? [??????]|???? Hred]; subst; auto.
-  destruct (Hred Δ (m ∪ mA) (InExpr ∅ mA)); auto; [|inv_rcstep].
-  constructor; eauto. by rewrite sep_right_id by auto.
+    inversion 1 as [|??? [??????]|???? Hred]; subst; try by auto.
+  destruct (Hred Δ n (m ∪ mA) (InExpr ∅ mA)); auto.
+  * constructor; eauto using assert_weaken. by rewrite sep_right_id by auto.
+  * inv_rcstep.
 Qed.
 
 (** The lemma [ax_expr_compose] is used to prove the structural Hoare rules for
@@ -385,44 +392,47 @@ Lemma ax_call_compose Γ δ A P Q (E : ectx K) E' ρ Δ n φ k m1 m2 :
   ⊥ [m1; m2] → ✓{Γ,Δ} m1 → ✓{Γ,Δ} m2 →
   ax_graph (ax_expr_cond ρ A) P Γ δ Δ ρ n (k ++ [CFun E]) φ m1 →
   (∀ Δ' n' m1' e',
-    n' ≤ n →
-    ⊥ [m1'; m2] → ✓{Γ,Δ'} m1' → ✓{Γ,Δ'} m2 → Δ ⇒ₘ Δ' →
-    ax_expr_funframe Γ Δ' A ρ (m1' ∪ m2) →
+    ⊥ [m1'; m2] → ✓{Γ,Δ'} m1' → ✓{Γ,Δ'} m2 →
     locks (subst E e') ⊆ mem_locks m1' →
+    ax_expr_funframe Γ Δ' A ρ n' (m1' ∪ m2) →
     ax_graph (ax_expr_cond ρ A) P Γ δ Δ' ρ n' [] (Expr (subst E e')) m1' →
+    Δ ⇒ₘ Δ' → n' ≤ n →
     ax_graph (ax_expr_cond ρ A) Q Γ δ Δ' ρ n' []
       (Expr (subst E' e')) (m1' ∪ m2)) →
   ax_graph (ax_expr_cond ρ A) Q Γ δ Δ ρ n (k ++ [CFun E']) φ (m1 ∪ m2).
 Proof.
   intros ? HE; revert Δ k φ m1.
-  induction n as [|n IH]; intros Δ k φ m1 ??? Hax Hnext; [apply ax_O |].
+  induction n as [[|n] IH] using lt_wf_ind;
+    intros Δ k φ m1 ??? Hax Hnext; [apply ax_O |].
   inversion Hax as [| |???? Hred Hstep];
     clear Hax; subst; try discriminate_list_equality.
   apply ax_further.
-  { intros Δ' m' a ?? Hframe; inversion_clear Hframe;
+  { intros Δ' n' m' a ??? Hframe; inversion_clear Hframe;
       subst; try discriminate_list_equality; simplify_mem_disjoint_hyps.
-    destruct (Hred Δ' (m1 ∪ m2 ∪ mf) (InFun (m2 ∪ mf))) as [S' p]; auto.
+    destruct (Hred Δ' n' (m1 ∪ m2 ∪ mf) (InFun (m2 ∪ mf))) as [S' p]; auto.
     { rewrite <-sep_associative by auto; constructor; auto.
       intro; discriminate_list_equality. }
     apply (rcstep_call_inv _ _ _ E E' _ _ _ _ _ p); intros; subst; eauto. }
-  intros Δ' ?? S' ?? Hframe p; inversion_clear Hframe as [mA mf|mf]; subst;
+  intros Δ' n' ?? S' ??? Hframe p;
+    inversion_clear Hframe as [mA mf|mf]; subst;
     try discriminate_list_equality; simplify_mem_disjoint_hyps.
   pattern S'; apply (rcstep_call_inv _ _ _ _ E _ _ _ _ _ p).
   * intros k' φ' m' p' ?.
-    feed inversion (Hstep Δ' (m1 ∪ m2 ∪ mf) (InFun (m2 ∪ mf))
-      (State (k' ++ [CFun E]) φ' m')) as [? Δ'' ?? m1' ?? Hunframe];
+    feed inversion (Hstep Δ' n' (m1 ∪ m2 ∪ mf) (InFun (m2 ∪ mf))
+      (State (k' ++ [CFun E]) φ' m')) as [Δ'' ?? ? m1' ?? Hunframe];
       subst; trivial.
     { rewrite <-sep_associative by auto. constructor; auto.
       intro; discriminate_list_equality. }
     inversion_clear Hunframe as [|mA| |]; subst;
       try discriminate_list_equality; simplify_mem_disjoint_hyps.
-    apply mk_ax_next with Δ'' (m1' ∪ m2); eauto 6 using focus_locks_valid_union.
+    apply mk_ax_next with Δ'' (m1' ∪ m2), IH;
+      eauto 6 using focus_locks_valid_union.
     rewrite sep_associative by auto. constructor; auto.
     intro; discriminate_list_equality.
   * intros f v -> -> p' ?.
-    feed inversion (Hstep Δ' (m1 ∪ m2 ∪ mf) (InFun (m2 ∪ mf))
+    feed inversion (Hstep Δ' n' (m1 ∪ m2 ∪ mf) (InFun (m2 ∪ mf))
       (State [] (Expr (subst E (# v)%E))
-      (m1 ∪ m2 ∪ mf))) as [? Δ'' ?? m1' ?? Hunframe _ Hlocks];
+      (m1 ∪ m2 ∪ mf))) as [Δ'' ??? m1' ?? Hunframe _ Hlocks];
       subst; trivial.
     { rewrite <-sep_associative by auto. constructor; auto. }
     inversion_clear Hunframe as [|mA ? Hm| |];
@@ -438,22 +448,22 @@ Proof.
       rewrite !ectx_subst_locks; esolve_elem_of.
     + eapply Hnext; eauto. exists mA; auto.
 Qed.
-Lemma ax_expr_compose Γ δ n {vn} A (Ps : vec (vassert K) vn) (Q : vassert K)
-    Δ (E : ectx_full K vn) (es : vec (expr K) vn) (ρ : stack K)
+Lemma ax_expr_compose Γ δ {vn} A (Ps : vec (vassert K) vn) (Q : vassert K)
+    Δ (E : ectx_full K vn) (es : vec (expr K) vn) (ρ : stack K) n
     (ms : vec (mem K) vn) (τlrs : vec (lrtype K) vn) σlr :
   ✓ Γ → locks E = ∅ → ✓{Δ}* ρ →
   ⊥ ms → (∀ i, ✓{Γ,Δ} (ms !!! i)) →
-  ax_expr_funframe Γ Δ A ρ (⋃ ms) →
+  ax_expr_funframe Γ Δ A ρ n (⋃ ms) →
   (∀ i, locks (es !!! i) ⊆ mem_locks (ms !!! i)) →
   (∀ i, ax_graph (ax_expr_cond ρ A) (ax_expr_post (Ps !!! i) (τlrs !!! i))
       Γ δ Δ ρ n [] (Expr (es !!! i)) (ms !!! i)) →
-  (∀ Δ' (Ωs : vec _ vn) (νs : vec _ vn) (ms' : vec _ vn),
-    ⊥ ms' → (∀ i, ✓{Γ,Δ'} (ms' !!! i)) → Δ ⇒ₘ Δ' →
+  (∀ Δ' n' (Ωs : vec _ vn) (νs : vec _ vn) (ms' : vec _ vn),
+    ⊥ ms' → (∀ i, ✓{Γ,Δ'} (ms' !!! i)) → Δ ⇒ₘ Δ' → n' ≤ n →
     (∀ i, (Γ,Δ') ⊢ νs !!! i : τlrs !!! i) →
     (∀ i, mem_locks (ms' !!! i) = Ωs !!! i) →
     (∀ i,
-      assert_holds ((Ps !!! i) (νs !!! i)) Γ Δ' ρ (cmap_erase (ms' !!! i))) →
-    ax_graph (ax_expr_cond ρ A) (ax_expr_post Q σlr) Γ δ Δ' ρ n []
+      assert_holds ((Ps !!! i) (νs !!! i)) Γ Δ' ρ n' (cmap_erase (ms' !!! i))) →
+    ax_graph (ax_expr_cond ρ A) (ax_expr_post Q σlr) Γ δ Δ' ρ n' []
        (Expr (depsubst E (vzip_with EVal Ωs νs)%E)) (⋃ ms')) →
   ax_graph (ax_expr_cond ρ A) (ax_expr_post Q σlr) Γ δ Δ ρ n []
     (Expr (depsubst E es)) (⋃ ms).
@@ -466,14 +476,15 @@ Proof.
       intros i; specialize (Hax1 i); rewrite vlookup_zip_with in Hax1;
       (eapply ax_expr_lrval; [| |eauto]);
       eauto using ax_expr_funframe_weaken, @sep_subseteq_lookup. }
-  apply ax_further.
-  { intros Δ' ???? Hframe; inversion_clear Hframe;
-      simplify_equality'; simplify_mem_disjoint_hyps.
-    rewrite (ectx_full_to_item_correct _ _ i); apply (rcred_ectx _ _ [_]).
+  apply ax_further_alt.
+  intros Δ' n' m' a ??? Hframe; inversion_clear Hframe as [mA mf ??? Hm|];
+    simplify_equality'; simplify_mem_disjoint_hyps.
+  split; [|intros S' p].
+  { rewrite (ectx_full_to_item_correct _ _ i); apply (rcred_ectx _ _ [_]).
     assert (⊥ (ms !!! i :: delete (i:nat) (ms:list _) ++ [mf;mA])).
     { by rewrite app_comm_cons, sep_disjoint_equiv_delete. }
     eapply (ax_red (ax_expr_cond ρ A) (ax_expr_post (Ps !!! i) (τlrs !!! i)))
-      with Δ' n (ms !!! i) (InExpr (⋃ delete (i:nat) (ms:list _) ∪ mf) mA).
+      with Δ' n' (ms !!! i) (InExpr (⋃ delete (i:nat) (ms:list _) ∪ mf) mA).
     { eauto using cmap_union_list_lookup_valid. }
     { econstructor; auto 1.
       { by rewrite sep_associative, sep_union_delete by auto. }
@@ -482,18 +493,16 @@ Proof.
         eauto using cmap_union_list_lookup_valid. }
     { simpl; contradict Hi; eauto using ax_expr_post_expr_nf. }
     eauto using ax_graph_weaken.  }
-  intros Δ' m' a S' ?? Hframe p; inversion_clear Hframe as [mA mf ??? Hm|];
-    simplify_equality'; simplify_mem_disjoint_hyps.
   pattern S'; apply (rcstep_expr_depsubst_inv _ _ _ _ _ _ _ _ p); clear p.
   * clear i Hi; intros i e' m2 p' ?.
     assert (⊥ (ms !!! i :: delete (i:nat) (ms:list _) ++ [mf;mA])).
     { by rewrite app_comm_cons, sep_disjoint_equiv_delete. }
     feed inversion (ax_step (ax_expr_cond ρ A)
       (ax_expr_post (Ps !!! i) (τlrs !!! i))
-      Γ δ Δ' ρ n [] (Expr (es !!! i)) (ms !!! i)
+      Γ δ Δ' ρ n' [] (Expr (es !!! i)) (ms !!! i)
       (ms !!! i ∪ ⋃ delete (i:nat) (ms:list _) ∪ mf ∪ mA)
       (InExpr (⋃ delete (i:nat) (ms:list _) ∪ mf) mA)
-      (State [] (Expr e') m2)) as [? Δ'' ?? m ?? Hunframe _]; subst; auto.
+      (State [] (Expr e') m2)) as [Δ'' ? n'' ? m ?? Hunframe _]; subst; auto.
     { eauto using cmap_union_list_lookup_valid. }
     { constructor; rewrite ?sep_associative by auto; auto.
       apply cmap_union_valid_2; auto.
@@ -515,7 +524,7 @@ Proof.
     rewrite <-sep_union_insert by auto.
     assert (⊥ (mf :: mA :: vinsert i m ms)).
     { rewrite sep_disjoint_equiv_insert; auto. }
-    apply IH; auto 1 with arith.
+    apply IH; auto.
     + eauto using indexes_valid_weaken.
     + intros j. destruct (decide (i = j)); subst; [by rewrite !vlookup_insert|].
       rewrite vlookup_insert_ne by done.
@@ -525,13 +534,12 @@ Proof.
       by rewrite !vlookup_insert_ne.
     + intros j; destruct (decide (i = j)); subst; [by rewrite !vlookup_insert|].
       rewrite !vlookup_insert_ne by done.
-      apply ax_S, ax_graph_weaken with Δ; eauto.
-    + intros Δ''' Ωs vs ms' ??????. apply ax_S, Hax2; auto.
+      apply ax_graph_weaken with Δ (S n); eauto.
   * clear i Hi. intros i E' Ω f τs τ Ωs vs ? Hesi p ?.
     assert (Ω ∪ ⋃ Ωs ⊆ mem_locks (ms !!! i)) as HΩ.
     { transitivity (locks (es !!! i)); [|done].
       rewrite Hesi, ectx_subst_locks; simpl.
-      rewrite fmap_zip_with_l by auto with lia; clear; solve_elem_of. }
+      rewrite fmap_zip_with_l by auto; clear; solve_elem_of. }
     assert (⊥ (mf :: mA :: ms !!! i :: delete (i:nat) (ms:list _))).
     { rewrite sep_disjoint_equiv_delete by auto; auto. }
     assert (⊥ (mf :: mA ::
@@ -539,10 +547,10 @@ Proof.
     { rewrite <-mem_unlock_disjoint_le by auto; auto. }
     feed inversion (ax_step (ax_expr_cond ρ A)
       (ax_expr_post (Ps !!! i) (τlrs !!! i))
-      Γ δ Δ' ρ n [] (Expr (es !!! i)) (ms !!! i)
+      Γ δ Δ' ρ n' [] (Expr (es !!! i)) (ms !!! i)
       (⋃ ms ∪ mf ∪ mA) (InExpr (⋃ delete (i:nat) (ms:list _) ∪ mf) mA)
       (State [CFun E'] (Call f vs) (mem_unlock (Ω ∪ ⋃ Ωs) (⋃ ms ∪ mf ∪ mA))))
-      as [? Δ'' ?? m ?? Hunframe _ ? Hm']; trivial; subst.
+      as [Δ'' ? n'' ? m ?? Hunframe _ ? Hm']; trivial; subst.
     { eauto using cmap_union_list_lookup_valid. }
     { constructor; auto.
       { by rewrite sep_associative, sep_union_delete by auto. }
@@ -574,10 +582,10 @@ Proof.
       apply union_list_preserving, Forall2_fmap, Forall2_delete.
       apply Forall2_vlookup; auto. }
     { by rewrite (sep_commutative mA) by auto. }
-    intros Δ''' n' m' e' ????? HmA ? Hax; simplify_mem_disjoint_hyps.
+    intros Δ''' n''' m' e' ????? HmA ? Hax; simplify_mem_disjoint_hyps.
     rewrite <-sep_union_insert by auto.
     rewrite subst_snoc, <-ectx_full_to_item_correct_alt.
-    apply IH; auto 1 with arith.
+    apply IH; auto.
     + eauto using indexes_valid_weaken.
     + rewrite sep_disjoint_equiv_insert; auto.
     + intros j; destruct (decide (i = j)); subst; [by rewrite !vlookup_insert|].
@@ -588,13 +596,11 @@ Proof.
       by rewrite !vlookup_insert_ne by done.
     + intros j; destruct (decide (i = j)); subst; [by rewrite !vlookup_insert|].
       rewrite !vlookup_insert_ne by done.
-      apply ax_graph_weaken with Δ; eauto using ax_le.
-    + intros Δ'''' Ωs' νs' ms' ??????.
-      apply ax_le with (S n); auto with arith.
+      apply ax_graph_weaken with Δ (S n); eauto.
   * rewrite Forall_vlookup; naive_solver.
   * clear i Hi. intros i E' e ? p ?.
     destruct (ax_step_undef (ax_expr_cond ρ A)
-      (ax_expr_post (Ps !!! i) (τlrs !!! i)) Γ δ Δ' ρ n [] (Expr (es !!! i))
+      (ax_expr_post (Ps !!! i) (τlrs !!! i)) Γ δ Δ' ρ n' [] (Expr (es !!! i))
       (ms !!! i) (⋃ ms ∪ mf ∪ mA)
       (InExpr (⋃ delete (i:nat) (ms:list _) ∪ mf) mA) [] (UndefExpr E' e)
       (⋃ ms ∪ mf ∪ mA));
@@ -607,50 +613,50 @@ Proof.
     apply cmap_union_list_valid, Forall_delete, Forall_vlookup;
       eauto using cmap_union_list_lookup_valid.
 Qed.
-Lemma ax_expr_compose_1 Γ δ n A P Q Δ (E : ectx_full K 1) e ρ m τlr σlr :
+Lemma ax_expr_compose_1 Γ δ A P Q Δ (E : ectx_full K 1) e ρ n m τlr σlr :
   ✓ Γ → locks E = ∅ → ✓{Δ}* ρ → ✓{Γ,Δ} m →
-  ax_expr_funframe Γ Δ A ρ m →
+  ax_expr_funframe Γ Δ A ρ n m →
   locks e ⊆ mem_locks m →
   ax_graph (ax_expr_cond ρ A) (ax_expr_post P τlr) Γ δ Δ ρ n [] (Expr e) m →
-  (∀ Δ' Ω ν m',
-    ✓{Γ,Δ'} m' → Δ ⇒ₘ Δ' → (Γ,Δ') ⊢ ν : τlr → mem_locks m' = Ω →
-    assert_holds (P ν) Γ Δ' ρ (cmap_erase m') →
-    ax_graph (ax_expr_cond ρ A) (ax_expr_post Q σlr) Γ δ Δ' ρ n []
+  (∀ Δ' n' Ω ν m',
+    ✓{Γ,Δ'} m' → Δ ⇒ₘ Δ' → n' ≤ n → (Γ,Δ') ⊢ ν : τlr → mem_locks m' = Ω →
+    assert_holds (P ν) Γ Δ' ρ n' (cmap_erase m') →
+    ax_graph (ax_expr_cond ρ A) (ax_expr_post Q σlr) Γ δ Δ' ρ n' []
        (Expr (depsubst E [# %#{Ω} ν]%E)) m') →
   ax_graph (ax_expr_cond ρ A) (ax_expr_post Q σlr) Γ δ Δ ρ n []
     (Expr (depsubst E [# e])) m.
 Proof.
   intros ??????? Hax. rewrite <-(sep_right_id m) by auto.
-  apply (ax_expr_compose Γ δ n A [# P]%A _ Δ E [# e] ρ [# m] [# τlr]); simpl;
+  apply (ax_expr_compose Γ δ A [# P]%A _ Δ E [# e] ρ n [# m] [# τlr]); simpl;
     rewrite ?sep_right_id by auto; auto; try (by intros; inv_all_vec_fin).
-  intros Δ' Ωs νs ms' ? Hm' ? Hν Hlocks Hax'; inv_all_vec_fin; simpl.
+  intros Δ' n' Ωs νs ms' ? Hm' ?? Hν Hlocks Hax'; inv_all_vec_fin; simpl.
   apply Hax; simpl; rewrite ?sep_right_id by auto; auto;
     apply (Hm' 0%fin) || apply (Hν 0%fin) ||
     apply (Hlocks 0%fin) || apply (Hax' 0%fin).
 Qed.
-Lemma ax_expr_compose_2 Γ δ n A P1 P2 Q Δ
-    (E : ectx_full K 2) e1 e2 ρ m1 m2 τlr1 τlr2 σlr :
+Lemma ax_expr_compose_2 Γ δ A P1 P2 Q Δ
+    (E : ectx_full K 2) e1 e2 ρ n m1 m2 τlr1 τlr2 σlr :
   ✓ Γ → locks E = ∅ → ✓{Δ}* ρ → ⊥ [m1; m2] → ✓{Γ,Δ} m1 → ✓{Γ,Δ} m2 →
-  ax_expr_funframe Γ Δ A ρ (m1 ∪ m2) →
+  ax_expr_funframe Γ Δ A ρ n (m1 ∪ m2) →
   locks e1 ⊆ mem_locks m1 → locks e2 ⊆ mem_locks m2 →
   ax_graph (ax_expr_cond ρ A) (ax_expr_post P1 τlr1) Γ δ Δ ρ n [] (Expr e1) m1 →
   ax_graph (ax_expr_cond ρ A) (ax_expr_post P2 τlr2) Γ δ Δ ρ n [] (Expr e2) m2 →
-  (∀ Δ' Ω1 Ω2 ν1 ν2 m1' m2',
-    ⊥ [m1';m2'] → ✓{Γ,Δ'} m1' → ✓{Γ,Δ'} m2' → Δ ⇒ₘ Δ' →
+  (∀ Δ' n' Ω1 Ω2 ν1 ν2 m1' m2',
+    ⊥ [m1';m2'] → ✓{Γ,Δ'} m1' → ✓{Γ,Δ'} m2' → Δ ⇒ₘ Δ' → n' ≤ n →
     (Γ,Δ') ⊢ ν1 : τlr1 → (Γ,Δ') ⊢ ν2 : τlr2 →
     mem_locks m1' = Ω1 → mem_locks m2' = Ω2 →
-    assert_holds (P1 ν1) Γ Δ' ρ (cmap_erase m1') →
-    assert_holds (P2 ν2) Γ Δ' ρ (cmap_erase m2') →
-    ax_graph (ax_expr_cond ρ A) (ax_expr_post Q σlr) Γ δ Δ' ρ n []
+    assert_holds (P1 ν1) Γ Δ' ρ n' (cmap_erase m1') →
+    assert_holds (P2 ν2) Γ Δ' ρ n' (cmap_erase m2') →
+    ax_graph (ax_expr_cond ρ A) (ax_expr_post Q σlr) Γ δ Δ' ρ n' []
        (Expr (depsubst E [# %#{Ω1} ν1; %#{Ω2} ν2]%E)) (m1' ∪ m2')) →
   ax_graph (ax_expr_cond ρ A) (ax_expr_post Q σlr) Γ δ Δ ρ n []
     (Expr (depsubst E [# e1; e2])) (m1 ∪ m2).
 Proof.
   intros ??????????? Hax. rewrite <-(sep_right_id m2) by auto.
-  apply (ax_expr_compose Γ δ n A [# P1; P2]%A Q Δ E
-    [# e1; e2] ρ [# m1; m2] [# τlr1; τlr2] σlr); simpl;
+  apply (ax_expr_compose Γ δ A [# P1; P2]%A Q Δ E
+    [# e1; e2] ρ n [# m1; m2] [# τlr1; τlr2] σlr); simpl;
     rewrite ?sep_right_id by auto; auto; try (by intros; inv_all_vec_fin).
-  intros Δ' Ωs νs ms' ? Hm' ? Hν Hlocks Hax'; inv_all_vec_fin; simpl.
+  intros Δ' n' Ωs νs ms' ? Hm' ?? Hν Hlocks Hax'; inv_all_vec_fin; simpl.
   apply Hax; simpl; rewrite ?sep_right_id by auto; auto;
     repeat match goal with
     | H : ∀ _ : fin _, _ |- _ => apply (H 0%fin)
