axiomatic_graph.v
@@ -1,36 +1,43 @@
 (* Copyright (c) 2012-2015, Robbert Krebbers. *)
 (* This file is distributed under the terms of the BSD license. *)
 Require Export restricted_smallstep memory_separation type_system.
-Local Hint Extern 1 (_ ⊥ _) => solve_sep_disjoint.
-Local Hint Extern 1 (⊥ _) => solve_sep_disjoint.
 
 Record ax_frame_cond (K : Set) `{Env K} (A : Type) : Type := {
-  frame : env K → memenv K → ctx K → focus K → mem K → mem K → A → Prop;
-  unframe : env K → memenv K → ctx K → focus K → mem K → mem K → A → Prop;
-  frame_valid Γ Δ k φ m m' a :
-    ✓ Γ → frame Γ Δ k φ m m' a → ✓{Γ,Δ} m → ✓{Γ,Δ} m';
-  unframe_valid Γ Δ k φ m m' a :
-    ✓ Γ → unframe Γ Δ k φ m m' a → ✓{Γ,Δ} m' → ✓{Γ,Δ} m
+  frame :
+    env K → memenv K → ctx K → nat → focus K → mem K → mem K → A → Prop;
+  unframe :
+    env K → memenv K → ctx K → nat → focus K → mem K → mem K → A → Prop;
+  frame_valid Γ Δ k n φ m m' a :
+    ✓ Γ → frame Γ Δ k n φ m m' a → ✓{Γ,Δ} m → ✓{Γ,Δ} m';
+  unframe_valid Γ Δ k n φ m m' a :
+    ✓ Γ → unframe Γ Δ k n φ m m' a → ✓{Γ,Δ} m' → ✓{Γ,Δ} m
 }.
-Arguments frame {_ _ _} _ _ _ _ _ _ _ _.
-Arguments unframe {_ _ _} _ _ _ _ _ _ _ _.
+Arguments frame {_ _ _} _ _ _ _ _ _ _ _ _.
+Arguments unframe {_ _ _} _ _ _ _ _ _ _ _ _.
 
 Record ax_assert (K : Set) `{Env K} : Type := {
-  ax_assert_holds : env K → memenv K → stack K → focus K → mem K → Prop;
-  ax_assert_weaken Γ1 Γ2 Δ1 Δ2 ρ φ m :
+  ax_assert_holds :
+    env K → memenv K → stack K → nat → focus K → mem K → Prop;
+  ax_assert_weaken Γ1 Γ2 Δ1 Δ2 ρ n n' φ m :
     ✓ Γ1 → ✓{Γ1,Δ1} m → ✓{Δ1}* ρ →
-    ax_assert_holds Γ1 Δ1 ρ φ m →
-    Γ1 ⊆ Γ2 → Δ1 ⇒ₘ Δ2 →
-    ax_assert_holds Γ2 Δ2 ρ φ m;
-  ax_assert_nf Γ δ Δ ρ φ m m' :
-    ax_assert_holds Γ Δ ρ φ m → nf (rcstep Γ δ ρ) (State [] φ m')
+    ax_assert_holds Γ1 Δ1 ρ n φ m →
+    Γ1 ⊆ Γ2 → Δ1 ⇒ₘ Δ2 → n' ≤ n →
+    ax_assert_holds Γ2 Δ2 ρ n' φ m;
+  ax_assert_nf Γ δ Δ ρ n φ m m' :
+    ax_assert_holds Γ Δ ρ n φ m → nf (rcstep Γ δ ρ) (State [] φ m')
 }.
-Arguments ax_assert_holds {_ _} _ _ _ _ _ _.
-Arguments ax_assert_nf {_ _} _ _ _ _ _ _ _ _ _ _.
+Arguments ax_assert_holds {_ _} _ _ _ _ _ _ _.
+Arguments ax_assert_nf {_ _} _ _ _ _ _ _ _ _ _ _ _.
 
 Section ax_graph.
 Context `{EnvSpec K}.
 Implicit Types Γ : env K.
+Implicit Types Δ : memenv K.
+Implicit Types m : mem K.
+
+Hint Extern 1 (_ ⊥ _) => solve_sep_disjoint.
+Hint Extern 1 (⊥ _) => solve_sep_disjoint.
+Hint Extern 1 (_ ≤ _) => omega.
 
 Section basics.
   Context {A} (F: ax_frame_cond K A) (P: ax_assert K) (Γ: env K) (δ: funenv K).
@@ -41,22 +48,22 @@ Section basics.
        nat → ctx K → focus K → mem K → Prop :=
     | ax_O k φ m : ax_graph Δ ρ 0 k φ m
     | ax_done n φ m :
-       ax_assert_holds P Γ Δ ρ φ m → ax_graph Δ ρ n [] φ m
+       ax_assert_holds P Γ Δ ρ n φ m → ax_graph Δ ρ n [] φ m
     | ax_further n k φ m :
-       (∀ Δ' m' a,
-         ✓{Γ,Δ'} m → Δ ⇒ₘ Δ' →
-         frame F Γ Δ' k φ m m' a →
+       (∀ Δ' n' m' a,
+         ✓{Γ,Δ'} m → Δ ⇒ₘ Δ' → n' < n →
+         frame F Γ Δ' k n' φ m m' a →
          red (rcstep Γ δ ρ) (State k φ m')) →
-       (∀ Δ' m' a S',
-         ✓{Γ,Δ'} m → Δ ⇒ₘ Δ' →
-         frame F Γ Δ' k φ m m' a →
+       (∀ Δ' n' m' a S',
+         ✓{Γ,Δ'} m → Δ ⇒ₘ Δ' → n' < n →
+         frame F Γ Δ' k n' φ m m' a →
          Γ\ δ\ ρ ⊢ₛ State k φ m' ⇒ S' →
          dom indexset (SMem S') ∖ dom indexset m' ∩ dom indexset Δ' = ∅ →
-         ax_next Δ' ρ n a S') →
-       ax_graph Δ ρ (S n) k φ m
+         ax_next Δ' ρ n' a S') →
+       ax_graph Δ ρ n k φ m
   with ax_next (Δ : memenv K) (ρ : stack K) : nat → A → state K → Prop :=
-    | mk_ax_next n Δ' k φ m m' a :
-       unframe F Γ Δ' k φ m m' a →
+    | mk_ax_next Δ' k n φ m m' a :
+       unframe F Γ Δ' k n φ m m' a →
        maybe Undef φ = None →
        focus_locks_valid φ m →
        ✓{Γ,Δ'} m' → Δ ⇒ₘ Δ' →
@@ -69,72 +76,38 @@ Section basics.
     intros; destruct φ; simpl; auto.
     rewrite mem_locks_union by auto; solve_elem_of.
   Qed.
-  Lemma ax_graph_weaken Δ Δ' ρ n k φ m :
-    ✓ Γ → ✓{Γ,Δ} m → ✓{Δ}* ρ →
-    ax_graph Δ ρ n k φ m → Δ ⇒ₘ Δ' → ax_graph Δ' ρ n k φ m.
-  Proof. destruct 4; constructor; eauto using ax_assert_weaken. Qed.
-  Lemma ax_further_pred Δ ρ n k φ m :
-    (∀ Δ' m' a,
-      ✓{Γ,Δ'} m → Δ ⇒ₘ Δ' →
-      frame F Γ Δ' k φ m m' a →
-      red (rcstep Γ δ ρ) (State k φ m')) →
-    (∀ Δ' m' a S',
-      ✓{Γ,Δ'} m → Δ ⇒ₘ Δ' →
-      frame F Γ Δ' k φ m m' a →
-      Γ\ δ\ ρ ⊢ₛ State k φ m' ⇒ S' →
-      dom indexset (SMem S') ∖ dom indexset m' ∩ dom indexset Δ' = ∅ →
-      ax_next Δ' ρ (pred n) a S') →
-    ax_graph Δ ρ n k φ m.
-  Proof. destruct n; econstructor (by eauto). Qed.
-  Lemma ax_further_pred_alt Δ ρ n k φ m :
-    (∀ Δ' m' a,
-      ✓{Γ,Δ'} m → Δ ⇒ₘ Δ' →
-      frame F Γ Δ' k φ m m' a →
+  Lemma ax_further_alt Δ ρ n k φ m :
+    (∀ Δ' n' m' a,
+      ✓{Γ,Δ'} m → Δ ⇒ₘ Δ' → n' < n →
+      frame F Γ Δ' k n' φ m m' a →
       red (rcstep Γ δ ρ) (State k φ m') ∧
       ∀ S',
         Γ\ δ\ ρ ⊢ₛ State k φ m' ⇒ S' →
         dom indexset (SMem S') ∖ dom indexset m' ∩ dom indexset Δ' = ∅ →
-        ax_next Δ' ρ (pred n) a S') →
+        ax_next Δ' ρ n' a S') →
     ax_graph Δ ρ n k φ m.
-  Proof. intros; apply ax_further_pred; naive_solver. Qed.
-  Lemma ax_S Δ ρ n k φ m (Hax : ax_graph Δ ρ (S n) k φ m) : ax_graph Δ ρ n k φ m
-  with ax_next_S Δ ρ n a S' (Hax : ax_next Δ ρ (S n) a S') : ax_next Δ ρ n a S'.
+  Proof. intros; apply ax_further; naive_solver. Qed.
+  Lemma ax_graph_weaken Δ Δ' ρ n n' k φ m :
+    ✓ Γ → ✓{Γ,Δ} m → ✓{Δ}* ρ →
+    ax_graph Δ ρ n k φ m → Δ ⇒ₘ Δ' → n' ≤ n →
+    ax_graph Δ' ρ n' k φ m.
   Proof.
-    * inversion Hax; subst; [by apply ax_done|destruct n; [apply ax_O |]].
-      apply ax_further; eauto.
-    * inversion Hax; subst; econstructor; eauto.
+    intros ??? Hax ??. destruct Hax as [k φ m|n2 φ m|n2 k φ m Hred Hstep].
+    * replace n' with 0 by lia. constructor.
+    * apply ax_done; eauto using ax_assert_weaken.
+    * constructor; eauto with arith.
   Qed.
-  Lemma ax_plus_l Δ ρ n1 n2 k φ m :
-    ax_graph Δ ρ (n1 + n2) k φ m → ax_graph Δ ρ n2 k φ m.
-  Proof. induction n1; simpl; auto using ax_S. Qed.
-  Lemma ax_next_plus_l Δ ρ n1 n2 a S' :
-    ax_next Δ ρ (n1 + n2) a S' → ax_next Δ ρ n2 a S'.
-  Proof. induction n1; simpl; auto using ax_next_S. Qed.
-  Lemma ax_le Δ ρ n1 n2 k φ m :
-    ax_graph Δ ρ n2 k φ m → n1 ≤ n2 → ax_graph Δ ρ n1 k φ m.
-  Proof.
-    intros Hax ?. rewrite (Minus.le_plus_minus n1 n2), plus_comm in Hax by done.
-    eauto using ax_plus_l.
-  Qed.
-  Lemma ax_next_le Δ ρ n1 n2 a S :
-    ax_next Δ ρ n2 a S → n1 ≤ n2 → ax_next Δ ρ n1 a S.
-  Proof.
-    intros Hax ?. rewrite (Minus.le_plus_minus n1 n2), plus_comm in Hax;
-      eauto using ax_next_plus_l.
-  Qed.
-  Lemma ax_pred Δ ρ n k φ m :
-    ax_graph Δ ρ n k φ m → ax_graph Δ ρ (pred n) k φ m.
-  Proof. intros. eauto using ax_le with arith. Qed.
   Lemma ax_step Δ ρ n k φ m m' a S' :
-    ✓{Γ,Δ} m → frame F Γ Δ k φ m m' a →
+    ✓{Γ,Δ} m → frame F Γ Δ k n φ m m' a →
     Γ\ δ\ ρ ⊢ₛ State k φ m' ⇒ S' →
     dom indexset (SMem S') ∖ dom indexset m' ∩ dom indexset Δ = ∅ →
     ax_graph Δ ρ (S n) k φ m → ax_next Δ ρ n a S'.
   Proof.
-    inversion 5; subst; eauto. destruct (ax_assert_nf P Γ δ Δ ρ φ m m'); eauto.
+    inversion 5; subst; eauto.
+    destruct (ax_assert_nf P Γ δ Δ ρ (S n) φ m m'); eauto.
   Qed.
   Lemma ax_step_undef Δ ρ n k φ m m' a k' Su m'' :
-    ✓{Γ,Δ} m → frame F Γ Δ k φ m m' a →
+    ✓{Γ,Δ} m → frame F Γ Δ k n φ m m' a →
     Γ\ δ\ ρ ⊢ₛ State k φ m' ⇒ State k' (Undef Su) m'' →
     dom indexset m'' ∖ dom indexset m' ∩ dom indexset Δ = ∅ →
     ¬ax_graph Δ ρ (S n) k φ m.
@@ -143,8 +116,8 @@ Section basics.
     by feed inversion (ax_step Δ ρ n k φ m m' a (State k' (Undef Su) m'')).
   Qed.
   Lemma ax_red Δ ρ n k φ m m' a :
-    ✓{Γ,Δ} m → frame F Γ Δ k φ m m' a →
-    ¬ax_assert_holds P Γ Δ ρ φ m →
+    ✓{Γ,Δ} m → frame F Γ Δ k n φ m m' a →
+    ¬ax_assert_holds P Γ Δ ρ (S n) φ m →
     ax_graph Δ ρ (S n) k φ m →
     red (rcstep Γ δ ρ) (State k φ m').
   Proof. by inversion 4; subst; eauto. Qed.
@@ -153,18 +126,18 @@ End basics.
 (** The predicate [ax] can be composed. This property is used to prove the
 structural Hoare rules. *)
 Definition ax_compose_diagram {A B} (F : ax_frame_cond K A)
-    (G : ax_frame_cond K B) (Γ : env K) (k2 : ctx K) := ∀ Δ k1 φ m m' b,
+    (G : ax_frame_cond K B) (Γ : env K) (k2 : ctx K) := ∀ Δ k1 n φ m m' b,
   ✓{Γ,Δ} m →
-  frame G Γ Δ (k1 ++ k2) φ m m' b → ∃ a,
-  (** 1.) *) frame F Γ Δ k1 φ m m' a ∧
+  frame G Γ Δ (k1 ++ k2) n φ m m' b → ∃ a,
+  (** 1.) *) frame F Γ Δ k1 n φ m m' a ∧
   (** 2.) *) ∀ Δ' k1' φ' m2 m2',
     ✓{Γ,Δ'} m2' → Δ ⇒ₘ Δ' →
-    unframe F Γ Δ' k1' φ' m2 m2' a →
-    unframe G Γ Δ' (k1' ++ k2) φ' m2 m2' b.
+    unframe F Γ Δ' k1' n φ' m2 m2' a →
+    unframe G Γ Δ' (k1' ++ k2) n φ' m2 m2' b.
 Lemma ax_compose_diagram_diag {A} (F : ax_frame_cond K A) Γ :
   ax_compose_diagram F F Γ [].
 Proof.
-  intros Δ k1 φ m m' a; rewrite (right_id_L [] (++)); exists a; split; auto.
+  intros Δ k1 n φ m m' a; rewrite (right_id_L [] (++)); exists a; split; auto.
   by intros; rewrite (right_id_L [] (++)).
 Qed.
 Lemma ax_compose {A B} (F : ax_frame_cond K A) (G : ax_frame_cond K B)
@@ -173,25 +146,26 @@ Lemma ax_compose {A B} (F : ax_frame_cond K A) (G : ax_frame_cond K B)
   ax_compose_diagram F G Γ k2 →
   ✓{Γ,Δ} m →
   ax_graph F P Γ δ Δ (rlocals ρ k2) n k1 φ m →
-  (∀ Δ' φ' m',
-    ax_assert_holds P Γ Δ' (rlocals ρ k2) φ' m' →
-    ✓{Γ,Δ'} m' → Δ ⇒ₘ Δ' →
-    ax_graph G Q Γ δ Δ' ρ n k2 φ' m') →
+  (∀ Δ' n' φ' m',
+    ax_assert_holds P Γ Δ' (rlocals ρ k2) n' φ' m' →
+    ✓{Γ,Δ'} m' → Δ ⇒ₘ Δ' → n' ≤ n →
+    ax_graph G Q Γ δ Δ' ρ n' k2 φ' m') →
   ax_graph G Q Γ δ Δ ρ n (k1 ++ k2) φ m.
 Proof.
-  intros ?. revert Δ m k1 φ; induction n as [|n IH]; [intros; apply ax_O|].
+  intros ?. revert Δ m k1 φ.
+  induction n as [[|n] IH] using lt_wf_ind; [intros; apply ax_O|].
   intros Δ m k1 φ HF ? Hax Hnext.
   inversion Hax as [| |???? Hred Hstep]; subst; eauto.
   apply ax_further.
-  { intros Δ' m'' a ???.
-    destruct (HF Δ' k1 φ m m'' a) as (b&?&_); eauto using rcred_app. }
-  intros Δ' m'' a [k' φ' m'] ??? p ?.
-  destruct (HF Δ' k1 φ m m'' a) as (b&?&?); auto.
+  { intros Δ' n' m'' a ????.
+    destruct (HF Δ' k1 n' φ m m'' a) as (b&?&_); eauto using rcred_app. }
+  intros Δ' n' m'' a [k' φ' m'] ???? p ?.
+  destruct (HF Δ' k1 n' φ m m'' a) as (b&?&?); auto.
   destruct (cstep_app_suffix_of Γ δ ρ k1 k2 φ m'' (State k' φ' m'))
     as [k3 ?]; simplify_equality'; eauto.
-  feed inversion (Hstep Δ' m'' b (State k3 φ' m'))
-    as [n' Δ'' k'' φ'' m2' m2 a']; subst; auto using rcstep_app_inv.
-  econstructor; eauto 10 using ax_S, unframe_valid.
+  feed inversion (Hstep Δ' n' m'' b (State k3 φ' m'))
+    as [Δ'' n'' k'' φ'' m2' m2 a']; subst; auto using rcstep_app_inv.
+  econstructor; eauto 10 using unframe_valid.
 Qed.
 Lemma ax_compose_cons {A B} (F : ax_frame_cond K A) (G : ax_frame_cond K B)
     (P Q : ax_assert K) Γ δ Δ n φ ρ Ek m :
@@ -199,10 +173,10 @@ Lemma ax_compose_cons {A B} (F : ax_frame_cond K A) (G : ax_frame_cond K B)
   ax_compose_diagram F G Γ [Ek] →
   ✓{Γ,Δ} m →
   ax_graph F P Γ δ Δ (rlocals ρ [Ek]) n [] φ m →
-  (∀ Δ' φ' m',
-    ax_assert_holds P Γ Δ' (rlocals ρ [Ek]) φ' m' →
-    ✓{Γ,Δ'} m' → Δ ⇒ₘ Δ' →
-    ax_graph G Q Γ δ Δ' ρ n [Ek] φ' m') →
+  (∀ Δ' n' φ' m',
+    ax_assert_holds P Γ Δ' (rlocals ρ [Ek]) n' φ' m' →
+    ✓{Γ,Δ'} m' → Δ ⇒ₘ Δ' → n' ≤ n →
+    ax_graph G Q Γ δ Δ' ρ n' [Ek] φ' m') →
   ax_graph G Q Γ δ Δ ρ n [Ek] φ m.
 Proof. intros ?; by apply ax_compose. Qed.
 
@@ -210,18 +184,18 @@ Proof. intros ?; by apply ax_compose. Qed.
 conjunction rule. These abstract versions are used to prove the concrete rules
 for both the expression and statement judgment. *)
 Definition ax_frame_diagram {A B} (F: ax_frame_cond K A) (G: ax_frame_cond K B)
-    (Γ : env K) (mf : mem K) := ∀ Δ k φ m m' b,
+    (Γ : env K) (mf : mem K) := ∀ Δ k n φ m m' b,
   ⊥ [m; mf] → ✓{Γ,Δ} m → ✓{Γ,Δ} mf →
-  frame G Γ Δ k φ (m ∪ mf) m' b → ∃ a,
-  (** 1.) *) frame F Γ Δ k φ m m' a ∧
+  frame G Γ Δ k n φ (m ∪ mf) m' b → ∃ a,
+  (** 1.) *) frame F Γ Δ k n φ m m' a ∧
   (** 2.) *) ∀ Δ' k' φ' m2 m2',
-    unframe F Γ Δ' k' φ' m2 m2' a →
+    unframe F Γ Δ' k' n φ' m2 m2' a →
     ✓{Γ,Δ'} m2' → Δ ⇒ₘ Δ' →
-    unframe G Γ Δ' k' φ' (m2 ∪ mf) m2' b ∧ ⊥ [m2; mf].
+    unframe G Γ Δ' k' n φ' (m2 ∪ mf) m2' b ∧ ⊥ [m2; mf].
 Lemma ax_frame_diagram_empty {A} (F : ax_frame_cond K A) Γ :
   ✓ Γ → ax_frame_diagram F F Γ ∅.
 Proof.
-  intros ?????? a ??? Ha; exists a.
+  intros ??????? a ??? Ha; exists a.
   rewrite sep_right_id in Ha by solve_sep_disjoint.
   split; auto; intros Δ' k' φ' m2 m2' ???.
   assert (sep_valid m2) by eauto using cmap_valid_sep_valid, unframe_valid.
@@ -233,63 +207,75 @@ Lemma ax_frame {A B}(F : ax_frame_cond K A) (G : ax_frame_cond K B)
   ax_frame_diagram F G Γ mf →
   ⊥ [m; mf] → ✓{Γ,Δ} m → ✓{Γ,Δ} mf →
   ax_graph F P Γ δ Δ ρ n k φ m →
-  (∀ Δ' φ' m',
-    ⊥ [m'; mf] → ✓{Γ,Δ'} m' → ✓{Γ,Δ'} mf → Δ ⇒ₘ Δ' →
-    ax_assert_holds P Γ Δ' ρ φ' m' →
-    ax_assert_holds Q Γ Δ' ρ φ' (m' ∪ mf)) →
+  (∀ Δ' n' φ' m',
+    ⊥ [m'; mf] → ✓{Γ,Δ'} m' → ✓{Γ,Δ'} mf → Δ ⇒ₘ Δ' → n' ≤ n →
+    ax_assert_holds P Γ Δ' ρ n' φ' m' →
+    ax_assert_holds Q Γ Δ' ρ n' φ' (m' ∪ mf)) →
   ax_graph G Q Γ δ Δ ρ n k φ (m ∪ mf).
 Proof.
-  intros ? HFG. revert Δ m k φ. induction n as [|n IH]; [constructor |].
+  intros ? HFG. revert Δ m k φ.
+  induction n as [[|n] IH] using lt_wf_ind; [intros; apply ax_O|].
   intros Δ m k φ ??? Hax HPQ.
   inversion Hax as [| |???? Hred Hstep]; subst; eauto using ax_done.
   apply ax_further.
-  { intros Δ' m' a; rewrite cmap_union_valid by auto; intros [??] ??.
-    destruct (HFG Δ' k φ m m' a) as (b&?&_); eauto. }
-  intros Δ' m' a S'; rewrite cmap_union_valid by auto; intros [??] ?? p ?.
-  destruct (HFG Δ' k φ m m' a) as (b&?&Hunframe); auto.
-  feed inversion (Hstep Δ' m' b S') as [? Δ'' k' φ' m2' m2 ? τf']; subst; auto.
+  { intros Δ' n' m' a; rewrite cmap_union_valid by auto; intros [??] ???.
+    destruct (HFG Δ' k n' φ m m' a) as (b&?&_); eauto. }
+  intros Δ' n' m' a S'; rewrite cmap_union_valid by auto; intros [??] ?? p ??.
+  destruct (HFG Δ' k n' φ m m' a) as (b&?&Hunframe); auto.
+  feed inversion (Hstep Δ' n' m' b S')
+    as [Δ'' k' ? φ' m2' m2 ? τf']; subst; auto.
   destruct (Hunframe Δ'' k' φ' m2' m2 τf'); trivial.
   apply mk_ax_next with Δ'' (m2' ∪ mf); eauto 10 using @cmap_valid_subseteq,
     @sep_union_subseteq_r, unframe_valid, focus_locks_valid_union.
 Qed.
 
-Lemma ax_weaken {A} (F G: ax_frame_cond K A) (P Q: ax_assert K) Γ δ Δ ρ n k φ m:
-  ✓ Γ →
-  ✓{Γ,Δ} m →
+Lemma ax_weaken {A} (F G : ax_frame_cond K A)
+    (P Q : ax_assert K) Γ δ Δ ρ n n' k φ m :
+  ✓ Γ → ✓{Γ,Δ} m → ✓{Δ}* ρ →
   ax_graph F P Γ δ Δ ρ n k φ m →
-  (∀ Δ' k' φ' m2 m2' a,
-    ✓{Γ,Δ'} m2 → Δ ⇒ₘ Δ' →
-    frame G Γ Δ' k' φ' m2 m2' a →
-    frame F Γ Δ' k' φ' m2 m2' a) →
-  (∀ Δ' k' φ' m2 m2' a,
-    ✓{Γ,Δ'} m2' → Δ ⇒ₘ Δ' →
-    unframe F Γ Δ' k' φ' m2 m2' a →
-    unframe G Γ Δ' k' φ' m2 m2' a) →
-  (∀ Δ' φ' m',
-    ✓{Γ,Δ'} m' → Δ ⇒ₘ Δ' →
-    ax_assert_holds P Γ Δ' ρ φ' m' → ax_assert_holds Q Γ Δ' ρ φ' m') →
-  ax_graph G Q Γ δ Δ ρ n k φ m.
+  n' ≤ n →
+  (∀ Δ' k' n' φ' m2 m2' a,
+    ✓{Γ,Δ'} m2 →
+    frame G Γ Δ' k' n' φ' m2 m2' a →
+    Δ ⇒ₘ Δ' → n' ≤ n →
+    frame F Γ Δ' k' n' φ' m2 m2' a) →
+  (∀ Δ' k' n' φ' m2 m2' a,
+    ✓{Γ,Δ'} m2' →
+    unframe F Γ Δ' k' n' φ' m2 m2' a →
+    Δ ⇒ₘ Δ' → n' ≤ n →
+    unframe G Γ Δ' k' n' φ' m2 m2' a) →
+  (∀ Δ' n' φ' m',
+    ✓{Γ,Δ'} m' →
+    ax_assert_holds P Γ Δ' ρ n' φ' m' →
+    Δ ⇒ₘ Δ' → n' ≤ n →
+    ax_assert_holds Q Γ Δ' ρ n' φ' m') →
+  ax_graph G Q Γ δ Δ ρ n' k φ m.
 Proof.
-  intros ?; revert Δ k φ m. induction n as [|n]; [constructor |].
-  intros Δ k φ m ? Hax ???.
+  intros ?; revert Δ k n' φ m.
+  induction n as [[|n] IH] using lt_wf_ind; intros Δ k n' φ m ?? Hax ????.
+  { replace n' with 0 by lia. by intros; apply ax_O. }
   inversion Hax as [| |???? Hred Hstep]; subst; eauto using ax_done.
-  apply ax_further; eauto; intros Δ' m' a S' ??? p ?.
-  feed inversion (Hstep Δ' m' a S'); subst; eauto.
-  econstructor; eauto 15 using unframe_valid.
+  { apply ax_done. eapply ax_assert_weaken with _ _ (S n); eauto. }
+  apply ax_further; eauto.
+  { intros Δ' n'' m' a ????; eapply (Hred Δ' n'' m' a); eauto. }
+  intros Δ' n'' m' a S' ???? p ?.
+  feed inversion (Hstep Δ' n'' m' a S'); subst; eauto.
+  econstructor; eauto.
+  eapply (IH n''); eauto using unframe_valid, indexes_valid_weaken.
 Qed.
 
 (** The standard framing condition that just adds an arbitrary frame to the
 memory before each step and takes it off after. *)
 Program Definition ax_disjoint_cond : ax_frame_cond K (mem K) := {|
-  frame Γ Δ k φ m m' mf := m' = m ∪ mf ∧ ✓{Γ,Δ} mf ∧ ⊥ [m; mf];
-  unframe Γ Δ k φ m m' mf := m' = m ∪ mf ∧ ⊥ [m; mf]
+  frame Γ Δ k n φ m m' mf := m' = m ∪ mf ∧ ✓{Γ,Δ} mf ∧ ⊥ [m; mf];
+  unframe Γ Δ k n φ m m' mf := m' = m ∪ mf ∧ ⊥ [m; mf]
 |}.
 Next Obligation. auto using cmap_union_valid_2. Qed.
 Next Obligation. eauto using cmap_valid_subseteq, @sep_union_subseteq_l. Qed.
 Lemma ax_disjoint_cond_frame_diagram Γ mf :
   ✓ Γ → ax_frame_diagram ax_disjoint_cond ax_disjoint_cond Γ mf.
 Proof.
-  intros ? Δ k φ m m' mf' ??? (->&?&?). exists (mf ∪ mf'); split.
+  intros ? Δ k n φ m m' mf' ??? (->&?&?). exists (mf ∪ mf'); split.
   { split; split_ands; eauto using cmap_union_valid_2.
     by rewrite sep_associative by auto. }
   intros Δ' k' φ' m2 m2' [-> ?] ??; split; eauto.
@@ -298,6 +284,6 @@ Qed.
 Lemma ax_disjoint_compose_diagram Γ Ek :
   ax_compose_diagram ax_disjoint_cond ax_disjoint_cond Γ [Ek].
 Proof.
-  intros Δ k φ m ? mf ? (->&?&?); exists mf; split_ands; eauto. by split.
+  intros Δ k n φ m ? mf ? (->&?&?); exists mf; split_ands; eauto. by split.
 Qed.
 End ax_graph.
